specs/Spec.HKDF.fsti
@@ -24,3 +24,35 @@ val hkdf_expand:
               /\ length prk + length info + 1 + Hash.size_hash a + Hash.size_block a <= Hash.max_input a}
   -> len:size_nat{len < 255 * Hash.size_hash a} ->
   Tot (lbytes len)
+
+
+val hkdf_build_label:
+    secret: bytes
+  -> label: bytes{length label <= maxint U8}
+  -> context: bytes{length context <= maxint U8
+                 /\ numbytes U16 + numbytes U8 + length label + numbytes U8 + length context <= max_size_t}
+  -> len: nat{len <= maxint U16} ->
+  Tot (lbytes (numbytes U16 + numbytes U8 + length label + numbytes U8 + length context))
+
+
+val hkdf_expand_label:
+    a: Hash.algorithm
+  -> secret: bytes{length secret <= Hash.max_input a}
+  -> label: bytes{length label <= maxint U8}
+  -> context: bytes{
+    let size_hkdf_label = numbytes U16 + numbytes U8 + length label + numbytes U8 + length context in
+    length context <= maxint U8
+  /\ length secret + size_hkdf_label + 1 + Hash.size_hash a + Hash.size_block a <= Hash.max_input a}
+  -> len: nat{len <= maxint U16 /\ len < 255 * Hash.size_hash a} ->
+  Tot (lbytes len)
+
+
+val hkdf_expand_derive_secret:
+    a: Hash.algorithm
+  -> secret: bytes{length secret <= Hash.max_input a}
+  -> label: bytes{length label <= maxint U8}
+  -> context: bytes{
+    let size_hkdf_label = numbytes U16 + numbytes U8 + length label + numbytes U8 + Hash.size_hash a in
+    length context <= maxint U8
+  /\ length secret + size_hkdf_label + 1 + Hash.size_hash a + Hash.size_block a <= Hash.max_input a} ->
+  Tot (lbytes (Hash.size_hash a))
